\documentclass[11pt]{article}

\usepackage{times}
\usepackage{amsfonts}
\usepackage{amsmath}
\usepackage[psamsfonts]{amssymb}
\usepackage{latexsym}
\usepackage{color}
\usepackage{graphics}
\usepackage{enumerate}
\usepackage{amstext}
\usepackage{url}
\usepackage{epsfig}
\def\Kset{\mathbb{K}}
\def\Nset{\mathbb{N}}
\def\Qset{\mathbb{Q}}
\def\Rset{\mathbb{R}}
\def\Sset{\mathbb{S}}
\def\Zset{\mathbb{Z}}
\def\squareforqed{\hbox{\rlap{$\sqcap$}$\sqcup$}}
\def\qed{\ifmmode\squareforqed\else{\unskip\nobreak\hfil
\penalty50\hskip1em\null\nobreak\hfil\squareforqed
\parfillskip=0pt\finalhyphendemerits=0\endgraf}\fi}

\DeclareMathOperator*{\E}{\rm E}
\def\vcdim{\textnormal{VCdim}}

%\newcommand{\ignore}[1]{}
\newenvironment{solution}{\vspace{.25cm}\noindent{\it Solution:}}{}



\usepackage[dvipsnames]{xcolor}
\usepackage{tikz,graphicx,amsmath,amsfonts,amscd,amssymb,bm,cite,epsfig,epsf,url}
\usepackage[hang,flushmargin]{footmisc}
\usepackage[colorlinks=true,urlcolor=blue,citecolor=blue]{hyperref}
\usepackage{amsthm,multirow,wasysym,appendix}
\usepackage{mathrsfs}
\usepackage{array,subcaption} 
% \usepackage[small,bf]{caption}
\usepackage{bbm}
\usepackage{pgfplots}
\usetikzlibrary{spy}
\usepgfplotslibrary{external}
\usepgfplotslibrary{fillbetween}
\usetikzlibrary{arrows,automata}
\usepackage{thmtools}
\usepackage{blkarray} 
\usepackage{textcomp}
\usepackage[left=0.8in,right=1.0in,top=1.0in,bottom=1.0in]{geometry}


\usepackage{times}
\usepackage{amsfonts}
\usepackage{amsmath}
\usepackage{latexsym}
\usepackage{color}
\usepackage{graphics}
\usepackage{enumerate}
\usepackage{amstext}
\usepackage{blkarray}
\usepackage{url}
\usepackage{epsfig}
\usepackage{bm}
\usepackage{hyperref}
\hypersetup{
    colorlinks=true,
    linkcolor=blue,
    filecolor=magenta,      
    urlcolor=blue,
}
\usepackage{textcomp}
\usepackage[left=0.8in,right=1.0in,top=1.0in,bottom=1.0in]{geometry}
\usepackage{mathtools}
\usepackage{minted}



\input{macros}

\begin{document}

\noindent Professor Rio\\
EN.585.615.81.SP21 Mathematical Methods\\
Take Home Project 1\\
Johns Hopkins University\\
Student: Yves Greatti\\\

\section{Question 1}
The rates of change of $C_e$ (free), $F^{18}DG$,  and $C_m$ (trapped), $F^{18}DG$-$6$-$P$
in brain tissue  are given by the system of differential equations:
\begin{align*}
	\begin{cases}
		\frac{d}{dt} \, C_e  = k_1 C_p - (k_2 + k_3) C_e + k_4 C_m \\
		\frac{d}{dt} \, C_m = k_3 C_e -  k_4 C_m \\
	\end{cases}
\end{align*}
Rearranging the terms of the differential equations gives:
\begin{align*}
	\begin{cases}
		\frac{d}{dt} \, C_e  + (k_2 + k_3) C_e - k_4 C_m  &= k_1 C_p \\
		k_3 C_e + \frac{d}{dt} \, C_m + k_4 C_m  &= 0\\
	\end{cases}
\end{align*}

First, since initial concentrations are assumed to be $0$: $C_e(0) = C_m(0) = 0$ and thus:
\begin{align*}
\mathscr{L}\{ \frac{d}{dt} \, C_e  \} &= s \rnd{C}_e(s) - \rnd{C}_e(0) = s \rnd{C}_e(s) - 0 = s \rnd{C}_e(s) \\
\mathscr{L}\{ \frac{d}{dt} \, C_m  \} &= s \rnd{C}_m(s) - \rnd{C}_m(0) = s \rnd{C}_m(s) - 0 = s \rnd{C}_m(s) \\
\end{align*}

Next, we take the Laplace transform on both sides of the ODEs which gives:

\begin{align*}
	\begin{cases}
		(s + k_2 + k_3)  \rnd{C}_e(s)  - k_4 \rnd{C}_m(s) &= k_1 \rnd{C}_p(s) \\
		-k_3  \rnd{C}_e(s)  + (s + k_4) \rnd{C}_m(s) &=  0
	\end{cases}
\end{align*}
 In matrix form, we have:
\begin{align*}
 \MAT{s + k_2 + k_3 & -k_4 \\ -k_3 & s + k_4} \MAT{ \rnd{C}_e(s) \\  \rnd{C}_m(s)} &= \MAT{k_1 \rnd{C}_p(s)  \\ 0}
\end{align*}
Solving for $\rnd{C}_e(s)$ and $\rnd{C}_m(s)$, Cramer's rule gives us:

\begin{align*}
  \rnd{C}_e(s) &= \frac { \begin{vmatrix}
        k_1  \rnd{C}_p(s) & - k_4  \\
        0 & s + k_4  \\
      \end{vmatrix} } {D} ~
  \rnd{C}_m(s) = \frac { \begin{vmatrix}
        s + k_2 + k_3  & k_1 \rnd{C}_p(s)\\
        -k_3 & 0  \\
      \end{vmatrix} } {D} \\
\end{align*}

where D is the determinant:

\begin{align*}
\begin{vmatrix}
        s + k_2 + k_3  & - k_4  \\
        - k_3 & s + k_4  \\
      \end{vmatrix} &= (s + k_2 + k_3) (s+ k_4) - k_3 k_4 \\
      &= s^2 + (k_2 + k_3 + k_4 ) s + (k_2 + k_3) k_4 - k_3 k_4 \\
      &= s^2 + (k_2 + k_3 + k_4) s + k_2 k_4
\end{align*}

The roots of this quadratic expression are:
\begin{align*}
& r_1 = \frac{1}{2} \bigg [ - (k_2 + k_3 + k_4) - \sqrt{ (k_2 + k_3 + k_4)^2 - 4 k_2 k_4} \bigg] \\
& r_2 = \frac{1}{2} \bigg [ - (k_2 + k_3 + k_4) + \sqrt{ (k_2 + k_3 + k_4)^2 - 4 k_2 k_4} \bigg]
\end{align*}
And thus $D = (s - r_1) (s - r_2)$. We have an expression for $C_i$ as $\rnd{C}_i(s)= \rnd{C}_e(s) + \rnd{C}_m(s)$ in s-space, but we want an expression of $C_i$ in t-space.
Therefore we take the inverse Laplace transform of $\rnd{C}_i(s)$. But first, we need a nice form for $\rnd{C}_e(s)$ and $\rnd{C}_m(s)$ so we can
find their inverse Laplace transforms in a table.

\begin{align*}
  \rnd{C}_e(s) &= \frac { \begin{vmatrix}
        k_1  \rnd{C}_p(s) & - k_4  \\
        0 & s + k_4  \\
      \end{vmatrix} } {D} \\ 
  \rnd{C}_e(s) &= k_1  \rnd{C}_p(s) \frac { s + k_4 }  { (s-r_1) (s-r_2)} \\ 
\end{align*}

We will now determine the partial fraction expansion of $\rnd{C}_e(s)$:
\begin{align*}
	\frac { s + k_4 }  { (s - r_1) (s - r_2)} 	&= \frac{A} {s - r_1} + \frac{B} {s - r_2} \\
								&= \frac{A (s - r_2) + B (s - r_1)} { (s - r_1) (s - r_2) } \\
								&= \frac{ (A + B) s - A r_2 - B r_1} { (s - r_1) (s - r_2) } \\
\end{align*}
Equating on each side powers of s in the numerator:

\begin{flalign}
s^1 &: A + B = 1 \\
s^0 &: - A r_2 - B r_1 = k_4
\end{flalign}
from $(1)$ we have $B = 1 - A$ and substituting back into $(2)$:

\begin{align*}
& A (r_1 - r_2) - r_1 = k_4 \\
& A = \frac{k_4 + r_1} {r_1 - r_2} \\
& B = 1 - A = 1 -  \frac{k_4 + r_1} {r_1 - r_2} = - \frac{k_4 + r_2} { r_1 - r_2} \\
\end{align*}

Plugging back these values for A and B in $\rnd{C}_e(s)$:
\begin{align*}
  \rnd{C}_e(s) 	&= k_1  \frac{\rnd{C}_p(s)} {r_1 - r_2}  \bigg[   \frac{k_4 + r_1} {s - r_1}  -    \frac{k_4 + r_2} {s - r_2}  \bigg ]\\ 
  			&= k_1 \frac{k_4 + r_1}  {r_1 - r_2}  \frac{\rnd{C}_p(s)} {s - r_1} - k_1 \frac{k_4 + r_2}  {r_1 - r_2}  \frac{\rnd{C}_p(s)} {s - r_2} \\
\end{align*}

The Laplace transform of the convolution between two functions is the product of the Laplace transform of these functions (p 226 equation 5.58 Riley book):
\begin{equation*}
\mathscr{L} \{ \int_0^t f(t') g(t-t') dt' \}  = \rnd{f}(s) \rnd{g}(s)
\end{equation*}

Let $\rnd{f}(s) = \rnd{C}_p(s)$ and $\rnd{g}(s) = \frac{1} {s-r_1}$, and we have:
\begin{align*}
&	\mathscr{L}^{-1} \{ \rnd{f}(s) \} = \mathscr{L}^{-1} \{ \rnd{C}_p(s) \} = C_p(t) \\
&	\mathscr{L}^{-1} \{ \rnd{g}(s) \} = \mathscr{L}^{-1} \{  \frac{1} {s-r_1} \} = e^{r_1 t} \\
\end{align*}

Therefore:
\begin{equation*}
\mathscr{L} \{ \int_0^t  C_p(t')  e^{r_1 (t-t')} dt' \}  = \frac{\rnd{C}_p(s)} {s-r_1} 
\end{equation*}

\end{document}
