\documentclass[12pt,twoside]{article}
\usepackage[dvipsnames]{xcolor}
\usepackage{tikz,graphicx,amsmath,amsfonts,amscd,amssymb,mathrsfs, bm,cite,epsfig,epsf,url}
\usepackage[hang,flushmargin]{footmisc}
\usepackage[colorlinks=true,urlcolor=blue,citecolor=blue]{hyperref}
\usepackage{amsthm,multirow,wasysym,appendix}
\usepackage{array,subcaption} 
% \usepackage[small,bf]{caption}
\usepackage{bbm}
\usepackage{pgfplots}
\usetikzlibrary{spy}
\usepgfplotslibrary{external}
\usepgfplotslibrary{fillbetween}
\usetikzlibrary{arrows,automata}
\usepackage{thmtools}
\usepackage{blkarray} 
\usepackage{textcomp}
\usepackage[left=0.8in,right=1.0in,top=1.0in,bottom=1.0in]{geometry}


\usepackage{times}
\usepackage{amsfonts}
\usepackage{amsmath}
\usepackage{latexsym}
\usepackage{color}
\usepackage{graphics}
\usepackage{enumerate}
\usepackage{amstext}
\usepackage{blkarray}
\usepackage{url}
\usepackage{epsfig}
\usepackage{bm}
\usepackage{hyperref}
\hypersetup{
    colorlinks=true,
    linkcolor=blue,
    filecolor=magenta,      
    urlcolor=blue,
}
\usepackage{textcomp}
\usepackage[left=0.8in,right=1.0in,top=1.0in,bottom=1.0in]{geometry}
\usepackage{mathtools}
\usepackage{minted}



\input{macros}

\begin{document}

\noindent Professor Rio\\
EN.585.615.81.SP21 Mathematical Methods\\
Take Home Project 2\\
Johns Hopkins University\\
Student: Yves Greatti\\\

\section*{Question 1}

The rates of change of $C_e$ (free), $F^{18}DG$,  and $C_m$ (trapped), $F^{18}DG$-$6$-$P$
in brain tissue  are given by the system of differential equations:
\begin{align*}
	\begin{cases}
		\frac{d}{dt} \, C_e  = k_1 C_p - (k_2 + k_3) C_e + k_4 C_m \\
		\frac{d}{dt} \, C_m = k_3 C_e -  k_4 C_m \\
	\end{cases}
\end{align*}
Rearranging the terms of the differential equations gives:
\begin{align*}
	\begin{cases}
		\frac{d}{dt} \, C_e  + (k_2 + k_3) C_e - k_4 C_m  &= k_1 C_p \\
		- k_3 C_e + \frac{d}{dt} \, C_m + k_4 C_m  &= 0\\
	\end{cases}
\end{align*}

First, since initial concentrations are assumed to be zero: $C_e(0) = C_m(0) = 0$ and thus:
\begin{align*}
\mathscr{L}\{ \frac{d}{dt} \, C_e  \} &= s \rnd{C}_e(s) - \rnd{C}_e(0) = s \rnd{C}_e(s) - 0 = s \rnd{C}_e(s) \\
\mathscr{L}\{ \frac{d}{dt} \, C_m  \} &= s \rnd{C}_m(s) - \rnd{C}_m(0) = s \rnd{C}_m(s) - 0 = s \rnd{C}_m(s) \\
\end{align*}

Next, we take the Laplace transform on both sides of the ODEs which gives:

\begin{align*}
	\begin{cases}
		(s + k_2 + k_3)  \rnd{C}_e(s)  - k_4 \rnd{C}_m(s) &= k_1 \rnd{C}_p(s) \\
		-k_3  \rnd{C}_e(s)  + (s + k_4) \rnd{C}_m(s) &=  0
	\end{cases}
\end{align*}
 In matrix form, we have:
\begin{align*}
 \MAT{s + k_2 + k_3 & -k_4 \\ -k_3 & s + k_4} \MAT{ \rnd{C}_e(s) \\  \rnd{C}_m(s)} &= \MAT{k_1 \rnd{C}_p(s)  \\ 0}
\end{align*}
Solving for $\rnd{C}_e(s)$ and $\rnd{C}_m(s)$, Cramer's rule gives us:

\begin{align*}
  \rnd{C}_e(s) &= \frac { \begin{vmatrix}
        k_1  \rnd{C}_p(s) & - k_4  \\
        0 & s + k_4  \\
      \end{vmatrix} } {D} ~
  \rnd{C}_m(s) = \frac { \begin{vmatrix}
        s + k_2 + k_3  & k_1 \rnd{C}_p(s)\\
        -k_3 & 0  \\
      \end{vmatrix} } {D} \\
\end{align*}

where D is the determinant:

\begin{align*}
\begin{vmatrix}
        s + k_2 + k_3  & - k_4  \\
        - k_3 & s + k_4  \\
      \end{vmatrix} &= (s + k_2 + k_3) (s+ k_4) - k_3 k_4 \\
      &= s^2 + (k_2 + k_3 + k_4 ) s + (k_2 + k_3) k_4 - k_3 k_4 \\
      &= s^2 + (k_2 + k_3 + k_4) s + k_2 k_4
\end{align*}

The roots of this quadratic expression are:
\begin{align*}
& r_1 = \frac{1}{2} \bigg [ - (k_2 + k_3 + k_4) - \sqrt{ (k_2 + k_3 + k_4)^2 - 4 k_2 k_4} \bigg] \\
& r_2 = \frac{1}{2} \bigg [ - (k_2 + k_3 + k_4) + \sqrt{ (k_2 + k_3 + k_4)^2 - 4 k_2 k_4} \bigg]
\end{align*}
And thus $D = (s - r_1) (s - r_2)$. We have an expression for $C_i$ as $\rnd{C}_i(s)= \rnd{C}_e(s) + \rnd{C}_m(s)$ in s-space, but we want an expression of $C_i$ in t-space.
Therefore we take the inverse Laplace transform of $\rnd{C}_i(s)$. But first, we need a nice form for $\rnd{C}_e(s)$ and $\rnd{C}_m(s)$ so we can
find their inverse Laplace transforms in a table.

\begin{align*}
  \rnd{C}_e(s) &= \frac { \begin{vmatrix}
        k_1  \rnd{C}_p(s) & - k_4  \\
        0 & s + k_4  \\
      \end{vmatrix} } {D} \\ 
  \rnd{C}_e(s) &= k_1  \rnd{C}_p(s) \frac { s + k_4 }  { (s-r_1) (s-r_2)} \\ 
\end{align*}

We will now determine the partial fraction expansion of $\rnd{C}_e(s)$:
\begin{align*}
	\frac { s + k_4 }  { (s - r_1) (s - r_2)} 	&= \frac{A} {s - r_1} + \frac{B} {s - r_2} \\
								&= \frac{A (s - r_2) + B (s - r_1)} { (s - r_1) (s - r_2) } \\
								&= \frac{ (A + B) s - A r_2 - B r_1} { (s - r_1) (s - r_2) } \\
\end{align*}
Equating on each side, coefficients for the same powers of s in the numerator:

\begin{flalign}
s^1 &: A + B = 1 \\
s^0 &: - A r_2 - B r_1 = k_4
\end{flalign}
from $(1)$ we have $B = 1 - A$ and substituting back into $(2)$:

\begin{align*}
& A (r_1 - r_2) - r_1 = k_4 \\
& A = \frac{k_4 + r_1} {r_1 - r_2} \\
& B = 1 - A = 1 -  \frac{k_4 + r_1} {r_1 - r_2} = - \frac{k_4 + r_2} { r_1 - r_2} \\
\end{align*}

Plugging back these values for A and B in $\rnd{C}_e(s)$:
\noindent
\begin{align*}
  \rnd{C}_e(s) 	&= k_1  \frac{\rnd{C}_p(s)} {r_1 - r_2}  \bigg[   \frac{k_4 + r_1} {s - r_1}  -    \frac{k_4 + r_2} {s - r_2}  \bigg ]\\ 
  			&= k_1 \frac{k_4 + r_1}  {r_1 - r_2}  \frac{\rnd{C}_p(s)} {s - r_1} - k_1 \frac{k_4 + r_2}  {r_1 - r_2}  \frac{\rnd{C}_p(s)} {s - r_2} \\
\end{align*}

The Laplace transform of the convolution between two functions is the product of the Laplace transform of these functions (p 227, equation 5.58 Riley book):
\begin{equation*}
  \mathscr{L}\{ (f * g) (t) \} = \mathscr{L} \{ \int_0^t f(t') g(t-t') dt' \}  = \rnd{f}(s) \rnd{g}(s)
\end{equation*}

Let $\rnd{f}(s) = \rnd{C}_p(s)$ and $\rnd{g}(s) = \frac{1} {s-r_1}$, we have:
\begin{align*}
&	\mathscr{L}^{-1} \{ \rnd{f}(s) \} = \mathscr{L}^{-1} \{ \rnd{C}_p(s) \} = C_p(t) \\
&	\mathscr{L}^{-1} \{ \rnd{g}(s) \} = \mathscr{L}^{-1} \{  \frac{1} {s-r_1} \} = e^{r_1 t} \\
\end{align*}

Therefore:
\begin{equation*}
\mathscr{L} \{ \int_0^t  C_p(t')  e^{r_1 (t-t')} dt' \}  = \frac{\rnd{C}_p(s)} {s-r_1} 
\end{equation*}

Taking the inverse Laplace transform on both side of the previous equation yields:
\begin{equation*}
	\int_0^t  C_p(t')  e^{r_1 (t-t')} dt'  = \mathscr{L}^{-1} \{  \frac{\rnd{C}_p(s)} {s-r_1} \}
\end{equation*}
Similarly, we have:
\begin{equation*}
	\int_0^t  C_p(t')  e^{r_2 (t-t')} dt'  = \mathscr{L}^{-1} \{  \frac{\rnd{C}_p(s)} {s-r_2} \}
\end{equation*}

We now take the inverse Laplace transform of $\rnd{C}_e(s)$ using the two previous expressions:
\begin{align*}
&	\mathscr{L}^{-1} \{ \rnd{C}_e(s) \} \\
& 	= C_e(t) \\
& 	= k_1 \frac{k_4 + r_1}  {r_1 - r_2}  \mathscr{L}^{-1} \{\frac{\rnd{C}_p(s)} {s - r_1} \} - k_1 \frac{k_4 + r_2}  {r_1 - r_2} \mathscr{L}^{-1} \{ \frac{\rnd{C}_p(s)} {s - r_2} \} \\
&	= k_1 \frac{k_4 + r_1}  {r_1 - r_2}   \int_0^t  C_p(t')  e^{r_1 (t-t')} dt' - k_1 \frac{k_4 + r_2}  {r_1 - r_2} \int_0^t  C_p(t')  e^{r_2 (t-t')} dt'  \\
\end{align*}

Next, we follow the same steps for $C_m(t)$:
\noindent
\begin{align*}
  \rnd{C}_m(s) 	&= k_1 k_3 \frac { \rnd{C}_p(s) } {(s-r_1) (s-r_2) }  \\
  			&= k_1 k_3   \frac { \rnd{C}_p(s) } {(r_1 - r_2) }  \bigg[ \frac{1} {s - r_1} - \frac{1} {s - r_2}  \bigg]\\
\mathscr{L}^{-1} \{ \rnd{C}_m(s) \} &= C_m(t) \\			
&= \frac{k_1 k_3} {r_1 - r_2} \bigg[ \mathscr{L}^{-1} \{  \frac{ \rnd{C}_p(s) } {s - r_1} \} - \mathscr{L}^{-1} \{  \frac{ \rnd{C}_p(s) } {s - r_2}  \} \bigg]\\
&=  \frac{k_1 k_3} {r_1 - r_2}    \int_0^t  C_p(t')  e^{r_1 (t-t')} dt' -  \frac{k_1 k_3} {r_1 - r_2}   \int_0^t  C_p(t')  e^{r_2 (t-t')} dt'  \\
\end{align*}

Putting all together:
\begin{align*}
	C_i(t)	&= C_e(t) + C_m(t) \\
			&= - ( \frac{ k_1 (k_4 + r_2)  + k_1 k_3  } { r_1 - r_2 } )  \int_0^t  C_p(t')  e^{r_2 (t-t')} dt'  + 
			\frac{ k_1 (k_4 + r_1)  + k_1 k_3  } { r_1 - r_2 } \int_0^t  C_p(t')  e^{r_1 (t-t')} dt' \\
			&= - (\frac{ k_1 } { r_1 - r_2 }) (k_3 + k_4 + r_2)  \int_0^t  C_p(t')  e^{r_2 (t-t')} dt'  + 
			 (\frac{ k_1 } { r_1 - r_2 }) (k_3 + k_4 + r_1)  \int_0^t  C_p(t')  e^{r_1 (t-t')} dt' \\
\end{align*}
 In the associated paper by Brooks:
\begin{equation*}
	\alpha_{1,2} = \frac{1}{2} \bigg [ k_2 + k_3 + k_4 \stackrel{-}{+} \sqrt{ (k_2 + k_3 + k_4)^2 - 4 k_2 k_4} \bigg ]
\end{equation*}
Thus:
\begin{align*}
	r_1 &= - \alpha_2  \\
	r_2 &= - \alpha_1 \\
\end{align*}
Substituting $\alpha_1$ and $\alpha_2$ into the expression we just obtained for $C_i(t)$ yields:
\begin{align*}
C_i(t)	&= \frac{ k_1 (k_3 + k_4 - \alpha_1) } { \alpha_1 - \alpha_2 }  \int_0^t e^{-\alpha_1 (t-t')}  C_p(t')   dt'  + 
		\frac{ k_1  ( \alpha_2 - k_3 - k_4) } { \alpha_1 - \alpha_2 }  \int_0^t e^{-\alpha_2 (t-t')}  C_p(t')   dt'  \\
		&= A  \int_0^t e^{-\alpha_1 (t-t')}  C_p(t')   dt'  + B \int_0^t e^{-\alpha_2 (t-t')}  C_p(t')   dt'  \\
		\text{with:} \\
&		A =  k_1 (k_3 + k_4 - \alpha_1) / (\alpha_1 - \alpha_2 )\\
&		B =  k_1 ( \alpha_2 - k_3 - k_4) / (\alpha_1 - \alpha_2) \\
\end{align*}
 We just have reproduced formula ($\textbf{4}$) in the associated paper by Brooks. Note that when $k_4 << k_2+k_3$, A and B reduces to:
\begin{align*}
& A \approx k_1 k_3 / (k_2 + k_3) \\
& B \approx k_1 k_2 / (k_2 + k_3) \\
\end{align*}

We can express the same expression of $C_i(t)$ in terms of convolutions (with definition of the convolution defined in p.227 equation 5.58 in Riley book):

\begin{equation*}
	C_i (t) = A (C_p(t) * e^{-\alpha_1 t}) + B  (C_p(t) * e^{-\alpha_2 t}) 
\end{equation*}

\end{document}
